Trying to improve Circle.v, does not compile at the moment

Coq/HIT/Circle.v
@@ -1,71 +1,84 @@
 Add LoadPath "..".
 Require Import Homotopy.
 
-(** For compatibility with Coq 8.2. *)
-Unset Automatic Introduction.
+(** The following should probably go somewhere in Paths.v. Hopefully it can
+   act as a good subtitute for the rewrite tactic. *)
 
-(** The circle type S^1, as a higher inductive type. *)
-
-Axiom circle : Type.
-
-Axiom base : circle.
-Axiom loop : base == base.
- 
-Axiom circle_rect :
-  forall (P : circle -> Type) (pt : P base) (lp : transport loop pt == pt), 
-    forall x : circle, P x.
-
-Axiom compute_base :
-  forall (P : circle -> Type) (pt : P base) (lp : transport loop pt == pt), 
-    circle_rect P pt lp base == pt.
-
-Axiom compute_loop :
-  forall (P : circle -> Type) (pt : P base) (lp : transport loop pt == pt), 
-    (! map (transport loop) (compute_base P pt lp)
-      @ (map_dep (circle_rect P pt lp) loop)
-      @ (compute_base P pt lp))
-    == lp.
-
-(** From this we can derive the non-dependent version of the
-   eliminator, with its propositional computation rules. *)
-
-Definition circle_rect' :
-  forall (B : Type) (pt : B) (lp : pt == pt), circle -> B.
+Lemma hrewrite {A : Type} (P : A -> Type) {x y : A} (p : x == y) : P y -> P x.
 Proof.
-  intros B pt lp.
-  apply circle_rect with (P := fun x => B) (pt := pt).
-  (* Since [pt] doesn't depend on [loop], the source [transport loop
-     pt] is equivalent to [pt].  The lemma which says this is
-     [trans_trivial], so it is tempting to write [apply
-     trans_trivial].  However, that would use it to solve the whole
-     goal, rather than allowing us to incorporate [lp] as well.  We
-     also need to be careful with our path-constructing tactics, lest
-     they overzealously use an identity path where we want to use a
-     nontrivial self-path. *)
-  apply @concat with (y := pt).
-  apply trans_trivial.
-  exact lp.
+  intro u.
+  induction p.
+  exact u.
 Defined.
 
-Definition compute_base' :
-  forall (B : Type) (pt : B) (lp : pt == pt),
-    circle_rect' B pt lp base == pt.
+Ltac hrewrite p :=
+  match type of p with
+    |  ?x == ?y  =>
+      pattern x ; apply (hrewrite _ p)
+  end.
+
+(** The circle type S^1, as a higher inductive type. We phrase it here
+   as a structure so that we can consider having two circles alter on. *)
+
+Structure circleStruct := mkCircle {
+  carrier :> Type ;
+  base : carrier ;
+  loop : base == base ;
+  circle_rect :
+  (forall (P : carrier -> Type) (pt : P base) (lp : transport loop pt == pt),
+    forall x : carrier, P x) ;
+  compute_base :
+  (forall (P : carrier -> Type) (pt : P base) (lp : transport loop pt == pt), 
+    circle_rect P pt lp base == pt);
+  compute_loop :
+  (forall (P : carrier -> Type) (pt : P base) (lp : transport loop pt == pt), 
+    map_dep (circle_rect P pt lp) loop
+    == map (transport loop) (compute_base P pt lp) @ lp @  (!compute_base P pt lp))
+}.
+
+Implicit Arguments base [c].
+Implicit Arguments loop [c].
+Implicit Arguments circle_rect [c].
+Implicit Arguments compute_base [c].
+Implicit Arguments compute_loop [c].
+
+Section NonDependent.
+
+  (** Next we construct the non-dependent version of the circle axioms. *)
+
+  Variable S1 : circleStruct.
+
+  Definition circle_rect' (B : Type) (pt : B) (lp : pt == pt) : S1 -> B.
+  Proof.
+    apply circle_rect with (P := fun _ => B) (pt := pt).
+    (* Since [pt] doesn't depend on [loop], the source [transport loop
+       pt] is equivalent to [pt].  The lemma which says this is
+       [trans_trivial], so it is tempting to write [apply
+       trans_trivial].  However, that would use it to solve the whole
+       goal, rather than allowing us to incorporate [lp] as well.  We
+       also need to be careful with our path-constructing tactics, lest
+       they overzealously use an identity path where we want to use a
+       nontrivial self-path. *)
+    hrewrite (trans_trivial (@loop S1) pt).
+    exact lp.
+Defined.
+
+Definition compute_base' (B : Type) (pt : B) (lp : pt == pt) :
+  circle_rect' B pt lp base == pt.
 Proof.
-  intros B pt lp.
   unfold circle_rect'.
-  apply compute_base with (P := fun x => B).
+  apply compute_base with (P := fun _ => B).
 Defined.
 
-Definition compute_loop' :
-  forall (B : Type) (pt : B) (lp : pt == pt),
-    (! (compute_base' B pt lp)
-      @ map (circle_rect' B pt lp) loop
-      @ (compute_base' B pt lp))
-    == lp.
+Definition compute_loop' (B : Type) (pt : B) (lp : pt == pt) :
+    map (circle_rect' B pt lp) loop ==
+    (compute_base' B pt lp) @ lp @ (!compute_base' B pt lp).
 Proof.
   intros B pt lp.
-  set (P := fun x : circle => B).
-  set (lp' := trans_trivial loop pt @ lp).
+  pose (P := fun _ : S1 => B).
+  pose (lp' := trans_trivial (@loop S1) pt @ lp).
+  unfold circle_rect'.
+  
   path_via (!compute_base P pt lp'
     @ !trans_trivial loop _
     @ map_dep (circle_rect P pt lp') loop
@@ -73,35 +86,50 @@ Proof.
   unwhisker.
   moveleft_onleft.
   apply opposite, map_dep_trivial.
-  path_via (!trans_trivial loop _
+  path_via (!trans_trivial loop  _
     @ (!map (transport loop) (compute_base P pt lp'))
     @ map_dep (circle_rect P pt lp') loop
     @ compute_base P pt lp').
   do_opposite_concat.
   associate_right.
   moveright_onleft.
-  associate_left.
+  moveright_left.
   apply compute_loop with (P := P) (pt := pt) (lp := lp').
 Defined.
 
+End NonDependent.
+
 (** If the circle is contractible, then UIP holds. *)
 
-Theorem circle_contr_implies_UIP : is_contr (circle) ->
+Theorem circle_contr_implies_UIP (S1 : circle) : is_contr S1 ->
   forall (A : Type) (x y : A) (p q : x == y), p == q.
+
 Proof.
   intros H A x y p q.
   induction p.
-  set (cq := circle_rect' A x q).
-  set (cqb := cq base).
-  set (cqcb := compute_base' A x q : cqb == x).
-  set (cql := map cq loop : cqb == cqb).
-  set (cqcl := compute_loop' A x q : (!cqcb @ cql @ cqcb == q)).
+  pose (cq := circle_rect' S1 A x q).
+  pose (cqb := cq base).
+  pose (cqcb := compute_base' S1 A x q : cqb == x).
+  pose (cql := map cq loop : cqb == cqb).
+  pose (cqcl := compute_loop' S1 A x q : (!cqcb @ cql @ cqcb == q)).
   path_via (!cqcb @ cql @ cqcb).
   moveleft_onright.
   moveleft_onleft.
   cancel_units.
   cancel_opposites.
   path_via (map cq (idpath base)).
-  apply contr_path2.
+  apply @contr_path2. 
   assumption.
 Defined.
+
+(* There is only one circle. *)
+
+Lemma one_circle (A : circle) (B : circle) : A <~> B.
+Proof.
+  exists (circle_rect' A B base loop).
+  apply hequiv_is_equiv with (g := circle_rect' B A base loop).
+  intro b.
+  path_via (@base B).
+  path_via (circle_rect' A B base loop ).
+
+  path_via b.
